src/cbor/pulse/raw/CBOR.Pulse.Raw.UTF8.fsti
@@ -1,0 +1,15 @@
+module CBOR.Pulse.Raw.UTF8
+include CBOR.Spec.API.UTF8
+open Pulse.Lib.Pervasives
+
+module U8 = FStar.UInt8
+module S = Pulse.Lib.Slice
+
+inline_for_extraction
+val impl_utf8_correct
+  (s: S.slice U8.t)
+  (#p: perm)
+  (#v: Ghost.erased (Seq.seq U8.t))
+: stt bool
+    (pts_to s #p v)
+    (fun res -> pts_to s #p v ** pure (res == correct v))
